\section{Stevens Operators}\label{stevens}

In the single ion
module {\prg so1ion} the operators are identified as shown below with $I_{\alpha}$.

\begin{eqnarray*}
X=J(J+1)\\
O_{00}&=&1\\
\hline
O_{11}&=&\frac{1}{2}[J_++J_-]=J_x=I_1 \\
O^s_{11}&=&\frac{-i}{2}[J_+-J_-]=J_y=I_2 \\
O_{10}&=&J_z=I_3 \\
\hline
O^s_{22}&=&\frac{-i}{2}[J_+^2-J_-^2]=J_xJ_y+J_yJ_x=2P_{xy}=I_4 \\
O^s_{21}&=&\frac{-i}{4}[J_z(J_+-J_-)+(J_+-J_-)J_z]=\frac{1}{2}[J_yJ_z+J_zJ_y]=P_{yz}=I_5 \\
O_{20}&=&[3J_z^2-X]=I_6 \\
O_{21}&=&\frac{1}{4}[J_z(J_++J_-)+(J_++J_-)J_z]=\frac{1}{2}[J_xJ_z+J_zJ_x]=P_{xz}=I_7 \\
O_{22}&=&\frac{1}{2}[J_+^2+J_-^2]=J_x^2-J_y^2 =I_8\\
\hline
O^s_{33}&=&\frac{-i}{2}[J_+^3-J_-^3]=I_9 \\
O^s_{32}&=&\frac{-i}{4}[(J_+^2-J_-^2)J_z+J_z(J_+^2-J_-^2)]=I_{10} \\
O^s_{31}&=&\frac{-i}{4}[(J_+-J_-)(5J_z^2-X-1/2)+(5J_z^2-X-1/2)(J_+-J_-)]=I_{11} \\
O_{30}&=&[5J_z^3-(3X-1)J_z]=I_{12} \\
O_{31}&=&\frac{1}{4}[(J_++J_-)(5J_z^2-X-1/2)+(5J_z^2-X-1/2)(J_++J_-)] =I_{13}\\
O_{32}&=&\frac{1}{4}[(J_+^2+J_-^2)J_z+J_z(J_+^2+J_-^2)]=I_{14} \\
O_{33}&=&\frac{1}{2}[J_+^3+J_-^3]=I_{15} \\
\hline
O^s_{44}&=&\frac{-i}{2}[(J_+^4-J_-^4]=I_{16}\\
O^s_{43}&=&\frac{-i}{4}[(J_+^3-J_-^3)J_z+J_z(J_+^3-J_-^3)] =I_{17}\\
O^s_{42}&=&\frac{-i}{4}[(J_+^2-J_-^2)(7J_z^2-X-5)+(7J_z^2-X-5)(J_+^2-J_-^2)]=I_{18} \\
O^s_{41}&=&\frac{-i}{4}[(J_+-J_-)(7J_z^3-(3X+1)J_z)+(7J_z^3-(3X+1)J_z)(J_+-J_-)]=I_{19} \\
O_{40}&=&[35J_z^4-(30X-25)J_z^2+3X^2-6X]=I_{20} \\
O_{41}&=&\frac{1}{4}[(J_++J_-)(7J_z^3-(3X+1)J_z)+(7J_z^3-(3X+1)J_z)(J_++J_-)]=I_{21} \\
O_{42}&=&\frac{1}{4}[(J_+^2+J_-^2)(7J_z^2-X-5)+(7J_z^2-X-5)(J_+^2+J_-^2)] =I_{22}\\
O_{43}&=&\frac{1}{4}[(J_+^3+J_-^3)J_z+J_z(J_+^3+J_-^3)]=I_{23} \\
O_{44}&=&\frac{1}{2}[(J_+^4+J_-^4]=I_{24}\\
\hline
O^s_{55}&=&\frac{-i}{2}[J_+^5-J_-^5]=I_{25} \\
O^s_{54}&=&\frac{-i}{4}[(J_+^4-J_-^4)J_z+J_z(J_+^4-J_-^4)]=I_{26} \\
O^s_{53}&=&\frac{-i}{4}[(J_+^3-J_-^3)(9J_z^2-X-33/2)+(9J_z^2-X-33/2)(J_+^3-J_-^3)]=I_{27} \\
O^s_{52}&=&\frac{-i}{4}[(J_+^2-J_-^2)(3J_z^3-(X+6)J_z)+(3J_z^3-(X+6)J_z)(J_+^2-J_-^2)]=I_{28}\\
O^s_{51}&=&\frac{-i}{4}[(J_+-J_-)\{21J_z^4-14J_z^2X+X^2-X+3/2\}+\{\dots\}(J_+-J_-)]=I_{29} \\
O_{50}&=&[63J_z^5-(70X-105)J_z^3+(15X^2-50X+12)J_z]=I_{30} \\
O_{51}&=&\frac{1}{4}[(J_++J_-)(21J_z^4-14J_z^2X+X^2-X+3/2)+(21J_z^4-14J_z^2X+X^2-X+3/2)(J_++J_-)]=I_{31} \\
O_{52}&=&\frac{1}{4}[(J_+^2+J_-^2)(3J_z^3-(X+6)J_z)+(3J_z^3-(X+6)J_z)(J_+^2+J_-^2)] =I_{32}\\
O_{53}&=&\frac{1}{4}[(J_+^3+J_-^3)(9J_z^2-X-33/2)+(9J_z^2-X-33/2)(J_+^3+J_-^3)]=I_{33} \\
O_{54}&=&\frac{1}{4}[(J_+^4+J_-^4)J_z+J_z(J_+^4+J_-^4)]=I_{34} \\
O_{55}&=&\frac{1}{2}[J_+^5+J_-^5]=I_{35} \\
\hline
O^s_{66}&=&\frac{-i}{2}[J_+^6-J_-^6]=I_{36}\\
O^s_{65}&=&\frac{-i}{4}[(J_+^5-J_-^5)J_z+J_z(J_+^5-J_-^5)] =I_{37}\\
O^s_{64}&=&\frac{-i}{4}[(J_+^4-J_-^4)(11J_z^2-X-38)+(11J_z^2-X-38)(J_+^4-J_-^4)]=I_{38} \\
O^s_{63}&=&\frac{-i}{4}[(J_+^3-J_-^3)(11J_z^3-(3X+59)J_z)+(11J_z^3-(3X+59)J_z)(J_+^3-J_-^3)]=I_{39} \\
O^s_{62}&=&\frac{-i}{4}[(J_+^2-J_-^2)\{33J_z^4-(18X+123)J_z^2+X^2+10X+102\}+\{\dots\}(J_+^2-J_-^2)]=I_{40} \\
O^s_{61}&=&\frac{-i}{4}[(J_+-J_-)\{33J_z^5-(30X-15)J_z^3+(5X^2-10X+12)J_z\}+\{\dots\}(J_+-J_-)]=I_{41} \\
O_{60}&=&[231J_z^6-(315X-735)J_z^4+(105X^2-525X+294)J_z^2-5X^3+40X^2-60X]=I_{42} \\
O_{61}&=&\frac{1}{4}[(J_++J_-)\{33J_z^5-(30X-15)J_z^3+(5X^2-10X+12)J_z\}+\{\dots\}(J_++J_-)]=I_{43} \\
O_{62}&=&\frac{1}{4}[(J_+^2+J_-^2)\{33J_z^4-(18X+123)J_z^2+X^2+10X+102\}+\{\dots\}(J_+^2+J_-^2)]=I_{44} \\
O_{63}&=&\frac{1}{4}[(J_+^3+J_-^3)(11J_z^3-(3X+59)J_z)+(11J_z^3-(3X+59)J_z)(J_+^3+J_-^3)]=I_{45} \\
O_{64}&=&\frac{1}{4}[(J_+^4+J_-^4)(11J_z^2-X-38)+(11J_z^2-X-38)(J_+^4+J_-^4)]=I_{46} \\
O_{65}&=&\frac{1}{4}[(J_+^5+J_-^5)J_z+J_z(J_+^5+J_-^5)]=I_{47} \\
O_{66}&=&\frac{1}{2}[J_+^6+J_-^6]=I_{48}\\
\end{eqnarray*}



